arrays/spec/contains.v
@@ -19,7 +19,7 @@ Module ContainsSpec (Params: SKIP_LIST_PARAMS).
   Section Proofs.
     Context `{!heapGS Σ, !gset_list_unionGS Σ, !lockG Σ}.
     
-    Theorem findPred_spec (key lvl: Z) (top_head curr: node_rep) (Skeys: gset Z) 
+    Theorem findPred_spec (lvl: nat) (key: Z) (top_head curr: node_rep) (Skeys: gset Z) 
       (bot: bot_gname) (top_sub: sub_gname) (bot_subs: list sub_gname) :
       {{{ 
         skip_list_equiv lvl top_head Skeys 1 bot (top_sub :: bot_subs)
@@ -57,8 +57,8 @@ Module ContainsSpec (Params: SKIP_LIST_PARAMS).
         { by iFrame "# ∗". }
         iIntros (pred succ) "(%Hrange' & #Hown_pred & #Hown_succ & _)".
 
-        wp_pures. case_bool_decide; wp_if.
-        - exfalso; assert (lvl = 0) by congruence; lia.
+        wp_pures. case_bool_decide as Hcase; wp_if.
+        - exfalso; inversion Hcase; lia.
         - wp_bind (Fst _).
           iInv (levelN lvl) as (S Skeys' L) "(Hinv_sub & _)" "Hclose".
           iDestruct "Hinv_sub" as "(>%Hperm & >%Hsort & >%Hequiv & >Hown_auth & >Hown_toks & Hlist)".
@@ -69,6 +69,7 @@ Module ContainsSpec (Params: SKIP_LIST_PARAMS).
             { iNext; iExists S, Skeys', L; by iFrame. }
 
             iModIntro; wp_pures.
+            assert (lvl - 1 = (lvl - 1)%nat) as -> by lia.
             iApply ("IH" with "[$] [] [%]").
             { by iLeft. }
             { lia. }
@@ -83,7 +84,7 @@ Module ContainsSpec (Params: SKIP_LIST_PARAMS).
             }
 
             rewrite list_equiv_invert_L; last done.
-            iDestruct "Hlist" as (s' succ' ? ? γ) "(>%Hsucc'_range & _ & Hpt' & #Hinvs' & Hs' & Hlock & HP & Himp)".
+            iDestruct "Hlist" as (γ s' h succ') "(>%Hsucc'_range & Hpt' & #Hinvs' & Hs' & Hlock & #Hlvl & HP & Himp)".
             iDestruct "HP" as"(>Hauth_pred & >Htoks_pred)".
 
             assert ({[ pred ]} = {[ pred ]} ⋅ {[ pred ]}) as -> by set_solver.
@@ -95,6 +96,7 @@ Module ContainsSpec (Params: SKIP_LIST_PARAMS).
             { iNext; iExists S, Skeys', L; by iFrame. }
 
             iModIntro; wp_pures.
+            assert (lvl - 1 = (lvl - 1)%nat) as -> by lia.
             iApply ("IH" with "[$] [Hauth_pred] [%]").
             { by iRight. }
             { lia. }
