arrays/spec/find.v
@@ -16,7 +16,7 @@ Module FindSpec (Params: SKIP_LIST_PARAMS).
   Export Invariant.
 
   Section Proofs.
-    Context `{!heapGS Σ, !gset_list_unionGS Σ, !lockG Σ} (lvl: Z).
+    Context `{!heapGS Σ, !gset_list_unionGS Σ, !lockG Σ} (lvl: nat).
     
     Theorem find_bot_spec (key: Z) (head curr: node_rep) (Skeys: gset Z) 
       (bot: bot_gname) (sub: sub_gname) :
@@ -83,7 +83,7 @@ Module FindSpec (Params: SKIP_LIST_PARAMS).
       destruct Lm as [|next Lm].
       - rewrite (list_equiv_split lvl curr succ ([head] ++ L)); last first.
         { rewrite app_ass -Hsplit_sep //. }
-        iDestruct "Hlist" as (γ s) "(Hpt & #Hs & #Hlock & Himp)".
+        iDestruct "Hlist" as (s) "(Hpt & #Hs & Himp)".
 
         wp_load.
         iPoseProof ("Himp" with "Hpt") as "Hlist".
@@ -173,7 +173,7 @@ Module FindSpec (Params: SKIP_LIST_PARAMS).
 
         rewrite (list_equiv_split lvl curr next ([head] ++ L)); last first.
         { rewrite app_ass -Hsplit_sep //. }
-        iDestruct "Hlist" as (γ n) "(Hpt & #Hn & #Hlock & Himp)".
+        iDestruct "Hlist" as (n) "(Hpt & #Hn & Himp)".
 
         wp_load.
         iPoseProof ("Himp" with "Hpt") as "Hlist".
@@ -243,7 +243,10 @@ Module FindSpec (Params: SKIP_LIST_PARAMS).
         ∗
         (own (s_auth sub) (◯ {[ succ ]}) ∨ ⌜ succ = tail ⌝)
         ∗
-        ∃ (γ: gname), is_lock γ (node_lock pred) (in_lock (node_next pred))
+        ∃ (γ: gname) (h: nat), 
+          ⌜ lvl < h ⌝
+          ∗
+          is_lock γ (node_lock pred) (in_lock (node_next pred) h)
       }}}.
     Proof.
       iIntros (Φ) "(#Hinv & Hown_curr & Hrange) HΦ".
@@ -271,7 +274,7 @@ Module FindSpec (Params: SKIP_LIST_PARAMS).
       }
 
       rewrite (list_equiv_invert); last done.
-      iDestruct "Hlist" as (s succ ? ? γ) "(>%Hsucc_range & _ & Hpt & #Hinvs & Hs & #Hlock & Himp)".
+      iDestruct "Hlist" as (γ s h succ) "(>%Hsucc_range & Hpt & #Hinvs & Hs & #Hlock & #Hlvl & Himp)".
       rewrite -elem_of_list_In Hperm elem_of_elements in Hsucc_range.
 
       wp_load.
@@ -297,7 +300,7 @@ Module FindSpec (Params: SKIP_LIST_PARAMS).
           iDestruct "Hown_frag" as "(? & ?)"; iLeft; iFrame.
         }
 
-        iExists γ. by iFrame "#".
+        iExists γ, h. iFrame "#".
       - iApply ("IH" $! succ with "[Hown_frag] [%]").
         {
           iRight.
@@ -311,6 +314,135 @@ Module FindSpec (Params: SKIP_LIST_PARAMS).
         { lia. }
 
         iNext; iApply "HΦ".
+    Qed.
+
+    Theorem findLock_spec (key: Z) (head curr: node_rep)
+      (sub: sub_gname) (obot: option bot_gname) (P: node_rep → iProp Σ) :
+      {{{ 
+        inv (levelN lvl) (lazy_list_inv lvl head sub obot P)
+        ∗
+        (⌜ curr = head ⌝ ∨ own (s_auth sub) (◯ {[ curr ]}))
+        ∗
+        ⌜ node_key curr < key < INT_MAX ⌝
+      }}}
+        findLock (rep_to_node curr) #key #lvl
+      {{{ pred succ, RET ((rep_to_node pred), (rep_to_node succ));
+        ⌜ node_key pred < key ≤ node_key succ ⌝
+        ∗
+        (⌜ pred = head ⌝ ∨ own (s_auth sub) (◯ {[ pred ]}))
+        ∗
+        (own (s_auth sub) (◯ {[ succ ]}) ∨ ⌜ succ = tail ⌝)
+        ∗
+        ∃ (γ: gname) (s: loc) (h: nat), 
+          ⌜ lvl < h ⌝
+          ∗
+          is_lock γ (node_lock pred) (in_lock (node_next pred) h)
+          ∗
+          in_lock (node_next pred) lvl
+          ∗
+          (node_next pred +ₗ lvl) ↦{#1 / 2} #s
+          ∗
+          inv (nodeN s) (node_inv s succ)
+          ∗
+          in_lock (node_next pred +ₗ lvl +ₗ 1) (h - 1 - lvl)
+          ∗
+          locked γ
+      }}}.
+    Proof.
+      iIntros (Φ) "(#Hinv & Hown_curr & Hrange) HΦ".
+      iRevert (curr) "Hown_curr Hrange".
+      iLöb as "IH". 
+      iIntros (curr) "#Hown_curr %Hrange".
+      
+      wp_lam. wp_let. wp_let.
+      wp_apply (find_sub_spec with "[Hown_curr]").
+      { by iFrame "#". }
+      iIntros (pred succ) "(%Hrange' & #Hown_pred & #Hown_succ & Hlock)".
+      iDestruct "Hlock" as (γ h) "(%Hlvl & #Hlock)".
+      wp_pures. wp_lam. wp_pures.
+
+      wp_bind (acquire _).
+      iApply (acquire_spec with "Hlock"); first done.
+      iNext; iIntros (v) "(Hin_lock & Hlocked)".
+      iDestruct "Hin_lock" as (vs) "(Hnext & %Hlength)".
+
+      pose proof (list_split vs (h - 1) lvl) as Hsplit.
+      destruct Hsplit as [next Hsplit]; try lia.
+      destruct Hsplit as [vs1 Hsplit]; destruct Hsplit as [vs2 Hsplit].
+      destruct Hsplit as [Hvs Hsplit]; destruct Hsplit as [Hlength1 Hlength2].
+
+      rewrite Hvs array_app array_cons Hlength1.
+      iDestruct "Hnext" as "(Hnext1 & Hnext & Hnext2)".
+
+      wp_pures. wp_lam. wp_pures.
+      wp_bind (Load #(node_next pred +ₗ lvl)).
+      iInv (levelN lvl) as (S Skeys L) "(Hinv_sub & Hmatch)" "Hclose".
+      iDestruct "Hinv_sub" as "(>%Hperm & >%Hsort & >%Hequiv & >Hown_auth & >Hown_toks & Hlist)".
+
+      iAssert (⌜ pred = head ∨ In pred L ⌝ ∗ ⌜ In succ L ∨ succ = tail ⌝)%I
+        with "[Hown_auth Hown_pred Hown_succ]" as "(%Hpred_range & %Hsucc_range)".
+      {
+        iSplit.
+        + iDestruct "Hown_pred" as "[Heq|Hown]"; first by iLeft.
+          iDestruct (own_valid_2 with "Hown_auth Hown") 
+            as %[Hvalid%gset_included]%auth_both_valid_discrete.
+          iPureIntro; right.
+          rewrite -elem_of_list_In Hperm elem_of_elements. 
+          set_solver.
+        + iDestruct "Hown_succ" as "[Hown|Heq]"; last by iRight.
+          iDestruct (own_valid_2 with "Hown_auth Hown") 
+            as %[Hvalid%gset_included]%auth_both_valid_discrete.
+          iPureIntro; left.
+          rewrite -elem_of_list_In Hperm elem_of_elements.
+          set_solver.
+      }
+
+      rewrite (list_equiv_invert lvl L head pred); last done.
+      iDestruct "Hlist" as (γ' s' h' succ') "(>%Hsucc'_in_L & >Hpt & #Hinvs' & >Hs' & _ & #Hlvl' & Himp)".
+      iDestruct (mapsto_agree with "Hnext Hpt") as %->.
+
+      wp_load.
+      iPoseProof ("Himp" with "[$]") as "Hlist".
+      iMod ("Hclose" with "[Hmatch Hlist Hown_auth Hown_toks]") as "_".
+      { iNext; iExists S, Skeys, L; by iFrame. }
+
+      iModIntro. wp_bind (Load _).
+      iInv (nodeN s') as "Hpt" "Hclose"; unfold node_inv.
+      wp_load.
+      iMod ("Hclose" with "Hpt") as "_".
+
+      iModIntro. wp_let. wp_lam. wp_pures. wp_lam. wp_pures.
+      case_bool_decide as Heq; wp_if.
+      + iModIntro; iApply "HΦ".
+        iFrame "# ∗".
+        iSplit; first done. iExists γ, s', h.
+
+        iAssert (in_lock (node_next pred) lvl) 
+          with "[Hnext1]" as "Hin_lock1".
+        { iExists vs1; by iFrame. }
+        iAssert (in_lock (node_next pred +ₗ lvl +ₗ 1) (h - 1 - lvl)) 
+          with "[Hnext2]" as "Hin_lock2".
+        { iExists vs2; by iFrame. }
+
+        assert (succ = succ') as <-; last by iFrame "# ∗".
+        apply (sorted_node_key_unique (L ++ [tail])).
+        - apply node_rep_sorted_app in Hsort; by destruct Hsort.
+        - by rewrite in_inv_rev.
+        - by rewrite in_inv_rev. 
+        - congruence.
+      + wp_lam. wp_pures.
+
+        iCombine "Hnext1 Hnext Hnext2" as "Hnext".
+        rewrite -Hlength1 -array_cons -array_app -Hvs.
+        iAssert (in_lock (node_next pred) h) 
+          with "[Hnext]" as "Hin_lock".
+        { iExists vs; by iFrame. }
+
+        wp_apply (release_spec with "[Hin_lock Hlocked]"); first done.
+        { iFrame "# ∗"; iExists succ'; iFrame. }
+        iIntros. wp_pures.
+        iApply ("IH" with "HΦ").
+        iFrame "#". iPureIntro; lia.
     Qed.
 
   End Proofs.
